Base.v
@@ -1,10 +1,10 @@
-Require Export Coq.Arith.Arith.
-Require Export Coq.ZArith.ZArith.
-Require Export Coq.NArith.NArith.
-Require Export Coq.PArith.PArith.
 Require Export Coq.Lists.List. Export ListNotations.
 Require Export Coq.Strings.Ascii.
 Require Export Coq.Strings.String.
+Require Export Coq.Arith.Arith.
+Require Export Coq.NArith.NArith.
+Require Export Coq.PArith.PArith.
+Require Export Coq.ZArith.ZArith.
 Require Export Coq.micromega.Lia.
 Require Export Coq.Program.Equality.
 Export IfNotations.
